<?xml version="1.0" encoding="UTF-8"?>
<rdf:RDF
   xmlns:dcterms="http://purl.org/dc/terms/"
   xmlns:ns1="http://www.opengis.net/def/metamodel/ogc-na/"
   xmlns:rdf="http://www.w3.org/1999/02/22-rdf-syntax-ns#"
   xmlns:rdfs="http://www.w3.org/2000/01/rdf-schema#"
   xmlns:skos="http://www.w3.org/2004/02/skos/core#"
>
  <rdf:Description rdf:about="http://www.opengis.net/def/profile/ogc/2.0/gml-sf0">
    <rdf:type rdf:resource="http://www.w3.org/2004/02/skos/core#Concept"/>
    <rdfs:label>Geography Markup Language (GML) Simple Features Compliance Level SF-0</rdfs:label>
    <dcterms:created rdf:datatype="http://www.w3.org/2001/XMLSchema#dateTime">2021-04-28T16:23:42.732904</dcterms:created>
    <ns1:status rdf:resource="http://www.opengis.net/def/status/valid"/>
    <rdfs:seeAlso rdf:resource="https://portal.ogc.org/files/?artifact_id=42729"/>
    <skos:definition>Compliance level SF-0 limits the property types of both spatial and non-spatial properties.</skos:definition>
    <skos:notation rdf:datatype="http://www.opengis.net/def/encoding/ogc/gml">gml-sf0</skos:notation>
    <skos:prefLabel>Geography Markup Language (GML) Simple Features Compliance Level SF-0</skos:prefLabel>
  </rdf:Description>
  <rdf:Description rdf:about="http://www.opengis.net/def/profile/ogc/2.0/gml-sf1">
    <rdf:type rdf:resource="http://www.w3.org/2004/02/skos/core#Concept"/>
    <rdfs:label>Geography Markup Language (GML) Simple Features Compliance Level SF-1</rdfs:label>
    <dcterms:created rdf:datatype="http://www.w3.org/2001/XMLSchema#dateTime">2021-04-28T16:23:42.733243</dcterms:created>
    <ns1:status rdf:resource="http://www.opengis.net/def/status/valid"/>
    <rdfs:seeAlso rdf:resource="https://portal.ogc.org/files/?artifact_id=42729"/>
    <skos:definition>Compliance level SF-1 supports everything in compliance level SF-0 but removes the restriction on value cardinality and allows user defined non-spatial property types to be used.</skos:definition>
    <skos:notation rdf:datatype="http://www.opengis.net/def/encoding/ogc/gml">gml-sf1</skos:notation>
    <skos:prefLabel>Geography Markup Language (GML) Simple Features Compliance Level SF-1</skos:prefLabel>
  </rdf:Description>
  <rdf:Description rdf:about="http://www.opengis.net/def/profile/ogc/2.0/gml-sf/">
    <rdf:type rdf:resource="http://www.w3.org/2004/02/skos/core#Collection"/>
    <rdfs:label>Levels of the Geography Markup Language (GML) simple features profile</rdfs:label>
    <ns1:status rdf:resource="http://www.opengis.net/def/status/valid"/>
    <skos:inScheme rdf:resource="http://www.opengis.net/def/profile/ogc/2.0/gml-sf"/>
    <skos:member rdf:resource="http://www.opengis.net/def/profile/ogc/2.0/gml-sf0"/>
    <skos:member rdf:resource="http://www.opengis.net/def/profile/ogc/2.0/gml-sf1"/>
    <skos:member rdf:resource="http://www.opengis.net/def/profile/ogc/2.0/gml-sf2"/>
    <skos:prefLabel>Levels of the Geography Markup Language (GML) simple features profile</skos:prefLabel>
  </rdf:Description>
  <rdf:Description rdf:about="http://www.opengis.net/def/profile/ogc/2.0/gml-sf">
    <rdf:type rdf:resource="http://www.w3.org/2004/02/skos/core#ConceptScheme"/>
    <rdfs:label>Levels of the Geography Markup Language (GML) simple features profile</rdfs:label>
    <ns1:collectionView rdf:resource="http://www.opengis.net/def/profile/ogc/2.0/gml-sf/"/>
    <ns1:status rdf:resource="http://www.opengis.net/def/status/valid"/>
    <skos:prefLabel>Levels of the Geography Markup Language (GML) simple features profile</skos:prefLabel>
    <dcterms:source>OGC Naming Authority on behalf of relevant OGC Working Group</dcterms:source>
  </rdf:Description>
  <rdf:Description rdf:about="http://www.opengis.net/def/ogc/">
    <skos:member rdf:resource="http://www.opengis.net/def/profile/ogc/2.0/gml-sf/"/>
  </rdf:Description>
  <rdf:Description rdf:about="http://www.opengis.net/def/profile/ogc/2.0/gml-sf2">
    <rdf:type rdf:resource="http://www.w3.org/2004/02/skos/core#Concept"/>
    <rdfs:label>Geography Markup Language (GML) Simple Features Compliance Level SF-2</rdfs:label>
    <dcterms:created rdf:datatype="http://www.w3.org/2001/XMLSchema#dateTime">2021-04-28T16:23:42.733569</dcterms:created>
    <ns1:status rdf:resource="http://www.opengis.net/def/status/valid"/>
    <rdfs:seeAlso rdf:resource="https://portal.ogc.org/files/?artifact_id=42729"/>
    <skos:definition>Compliance level SF-2 essentially corresponds to the OGC Simple Features specification. There are no restrictions placed on non-spatial properties but there are restrictions on spatial properties.</skos:definition>
    <skos:notation rdf:datatype="http://www.opengis.net/def/encoding/ogc/gml">gml-sf2</skos:notation>
    <skos:prefLabel>Geography Markup Language (GML) Simple Features Compliance Level SF-2</skos:prefLabel>
  </rdf:Description>
</rdf:RDF>
